aarch64+x64 spec: update specifications to use semi-lazy FPU switching
This includes extending the machine interface with new ops, adding the current
owner of the FPU state to the kernel state, and adding the new
seL4_TCB_Set_Flags syscall and related functions.

Signed-off-by: Corey Lewis <corey.lewis@proofcraft.systems>

spec/haskell/src/SEL4/API/Invocation.lhs
@@ -83,6 +83,10 @@ The following data type defines the set of possible TCB invocation operations. T
 >         | SetTLSBase {
 >             setTLSBaseTCB :: PPtr TCB,
 >             setTLSBaseNewBase :: Word }
+>         | SetFlags {
+>             setFlagsTCB :: PPtr TCB,
+>             setFlagsClear :: Word,
+>             setFlagsSet :: Word }
 >         deriving Show
 
 \subsubsection{CNode Invocations}
