spec/abstract/X64/ArchTcb_A.thy
@@ -11,7 +11,7 @@ Arch-specific functions for the abstract model of CSpace.
 chapter "Architecture-specific TCB functions"
 
 theory ArchTcb_A
-imports KHeap_A
+imports FPU_A
 begin
 
 context Arch begin arch_global_naming (A)
@@ -45,6 +45,17 @@ definition
   arch_post_modify_registers :: "obj_ref \<Rightarrow> obj_ref \<Rightarrow> (unit, 'a::state_ext) s_monad"
 where
   "arch_post_modify_registers cur t \<equiv> when (t \<noteq> cur) $ as_user t $ setRegister ErrorRegister 0"
+
+\<comment> \<open>The corresponding C code is not arch dependent and so is inline as part of invokeSetFlags\<close>
+definition arch_post_set_flags :: "obj_ref \<Rightarrow> tcb_flags \<Rightarrow> (unit, 'a::state_ext) s_monad" where
+  "arch_post_set_flags t flags \<equiv>
+     when (ArchFlag FpuDisabled \<in> flags) (fpu_release t)"
+
+definition arch_prepare_set_domain :: "obj_ref \<Rightarrow> domain \<Rightarrow> unit det_ext_monad" where
+  "arch_prepare_set_domain t new_dom \<equiv> do
+     cur_domain \<leftarrow> gets cur_domain;
+     when (cur_domain \<noteq> new_dom) $ fpu_release t
+   od"
 
 end
 end
